Move subst_transform to AbstractTransform

Launchbury/AbstractTransform.thy
@@ -4,17 +4,20 @@ begin
 
 
 locale AbstractAnalProp =
-  fixes PropApp :: "exp \<Rightarrow> var \<Rightarrow> 'a \<Rightarrow> ('a::cont_pt)"
-  fixes PropLam :: "var \<Rightarrow> exp \<Rightarrow> 'a \<Rightarrow> 'a"
-  fixes PropLetBody :: "heap \<Rightarrow> exp \<Rightarrow> 'a \<Rightarrow> 'a"
+  fixes PropApp :: "'a \<Rightarrow> ('a::cont_pt)"
+  fixes PropLam :: "'a \<Rightarrow> 'a"
+  fixes PropLetBody :: "'a \<Rightarrow> 'a"
   fixes PropLetHeap :: "heap \<Rightarrow> exp \<Rightarrow> 'a \<Rightarrow> (var \<Rightarrow> 'a\<^sub>\<bottom>)"
   assumes PropApp_eqvt: "\<pi> \<bullet> PropApp \<equiv> PropApp"
   assumes PropLam_eqvt: "\<pi> \<bullet> PropLam \<equiv> PropLam"
   assumes PropLetBody_eqvt: "\<pi> \<bullet> PropLetBody \<equiv> PropLetBody"
   assumes PropLetHeap_eqvt: "\<pi> \<bullet> PropLetHeap \<equiv> PropLetHeap"
 
+locale AbstractAnalPropSubst = AbstractAnalProp +
+  assumes PropLetHeap_subst:  "x \<notin> domA \<Gamma> \<Longrightarrow> y \<notin> domA \<Gamma> \<Longrightarrow> PropLetHeap (\<Gamma>[x::h=y]) (e[x::=y]) a = PropLetHeap \<Gamma> e a"
+
 locale AbstractTransform = AbstractAnalProp +
-  constrains PropApp :: "exp \<Rightarrow> var \<Rightarrow> 'a \<Rightarrow> ('a::pure_cont_pt)"
+  constrains PropApp :: "'a \<Rightarrow> ('a::pure_cont_pt)"
   fixes TransVar :: "'a \<Rightarrow> var \<Rightarrow> exp"
   fixes TransVar1 :: "'a \<Rightarrow> var \<Rightarrow> exp"
   fixes TransApp :: "'a \<Rightarrow> exp \<Rightarrow> var \<Rightarrow> exp"
@@ -29,13 +32,13 @@ locale AbstractTransform = AbstractAnalProp +
   assumes SuppTransLet: "supp (TransLet a ae \<Gamma> e) \<subseteq> supp (\<Gamma>, e) - atom ` domA \<Gamma>"
 begin
   nominal_function transform where
-    "transform a (App e x) = TransApp a (transform (PropApp e x a) e) x"
-  | "transform a (Lam [x]. e) = TransLam a x (transform (PropLam x e a) e)"
+    "transform a (App e x) = TransApp a (transform (PropApp a) e) x"
+  | "transform a (Lam [x]. e) = TransLam a x (transform (PropLam a) e)"
   | "transform a (Var x) = TransVar a x"
   | "transform a (Var1 x) = TransVar1 a x"
   | "transform a (Let \<Delta> e) = TransLet a  (PropLetHeap \<Delta> e a)
         (map_transform transform (PropLetHeap \<Delta> e a) \<Delta>)
-        (transform (PropLetBody \<Delta> e a) e)"
+        (transform (PropLetBody a) e)"
 proof-
 case goal1
   note PropApp_eqvt[eqvt_raw] PropLam_eqvt[eqvt_raw] PropLetBody_eqvt[eqvt_raw] PropLetHeap_eqvt[eqvt_raw] TransVar_eqvt[eqvt] TransVar1_eqvt[eqvt]  TransApp_eqvt[eqvt]  TransLam_eqvt[eqvt] TransLet_eqvt[eqvt]
@@ -66,27 +69,27 @@ case (goal9 a x e a' x' e')
   proof(rule eqvt_lam_case)
     fix \<pi> :: perm
 
-    have "supp (TransLam a x (transform_sumC (PropLam x e a, e))) \<subseteq> supp (Lam [x]. e)"
+    have "supp (TransLam a x (transform_sumC (PropLam a, e))) \<subseteq> supp (Lam [x]. e)"
       apply (rule subset_trans[OF SuppTransLam])
       apply (auto simp add:  exp_assn.supp supp_Pair supp_at_base pure_supp exp_assn.fsupp dest!: set_mp[OF supp_eqvt_at[OF goal9(1)], rotated])
       done
     moreover
     assume "supp \<pi> \<sharp>* (Lam [x]. e)" 
     ultimately
-    have *: "supp \<pi> \<sharp>* TransLam a x (transform_sumC (PropLam x e a, e))" by (auto simp add: fresh_star_def fresh_def)
+    have *: "supp \<pi> \<sharp>* TransLam a x (transform_sumC (PropLam a, e))" by (auto simp add: fresh_star_def fresh_def)
 
     note PropApp_eqvt[eqvt_raw] PropLam_eqvt[eqvt_raw] PropLetBody_eqvt[eqvt_raw] PropLetHeap_eqvt[eqvt_raw] TransVar_eqvt[eqvt] TransVar1_eqvt[eqvt]  TransApp_eqvt[eqvt]  TransLam_eqvt[eqvt] TransLet_eqvt[eqvt]
 
-    have "TransLam a (\<pi> \<bullet> x) (transform_sumC (PropLam (\<pi> \<bullet> x) (\<pi> \<bullet> e) a, \<pi> \<bullet> e))
-        = TransLam a (\<pi> \<bullet> x) (transform_sumC (\<pi> \<bullet>  (PropLam x e a, e)))"
+    have "TransLam a (\<pi> \<bullet> x) (transform_sumC (PropLam a, \<pi> \<bullet> e))
+        = TransLam a (\<pi> \<bullet> x) (transform_sumC (\<pi> \<bullet>  (PropLam a, e)))"
       by perm_simp rule
-    also have "\<dots> = TransLam a (\<pi> \<bullet> x) (\<pi> \<bullet> transform_sumC (PropLam x e a, e))"
+    also have "\<dots> = TransLam a (\<pi> \<bullet> x) (\<pi> \<bullet> transform_sumC (PropLam a, e))"
       unfolding eqvt_at_apply'[OF goal9(1)]..
-    also have "\<dots> = \<pi> \<bullet> (TransLam a x (transform_sumC (PropLam x e a, e)))"
+    also have "\<dots> = \<pi> \<bullet> (TransLam a x (transform_sumC (PropLam a, e)))"
       by simp
-    also have "\<dots> = TransLam a x (transform_sumC (PropLam x e a, e))"
+    also have "\<dots> = TransLam a x (transform_sumC (PropLam a, e))"
       by (rule perm_supp_eq[OF *])
-    finally show "TransLam a (\<pi> \<bullet> x) (transform_sumC (PropLam (\<pi> \<bullet> x) (\<pi> \<bullet> e) a, \<pi> \<bullet> e)) = TransLam a x (transform_sumC (PropLam x e a, e))" by simp
+    finally show "TransLam a (\<pi> \<bullet> x) (transform_sumC (PropLam a, \<pi> \<bullet> e)) = TransLam a x (transform_sumC (PropLam a, e))" by simp
   qed
 next
 case (goal18 a as body a' as' body')
@@ -104,20 +107,20 @@ case (goal18 a as body a' as' body')
   show ?case
   unfolding `a' = a`
   proof (rule eqvt_let_case)
-    have "supp (TransLet a  (PropLetHeap as body a) (map_transform (\<lambda>x0 x1. transform_sumC (x0, x1)) (PropLetHeap as body a) as) (transform_sumC (PropLetBody as body a, body))) \<subseteq> supp (Terms.Let as body)"
+    have "supp (TransLet a  (PropLetHeap as body a) (map_transform (\<lambda>x0 x1. transform_sumC (x0, x1)) (PropLetHeap as body a) as) (transform_sumC (PropLetBody a, body))) \<subseteq> supp (Let as body)"
       by (auto simp add: Let_supp supp_Pair pure_supp exp_assn.fsupp
                dest!: set_mp[OF supp_eqvt_at[OF goal18(2)], rotated] set_mp[OF SuppTransLet] set_mp[OF supp_map])
     moreover
     fix \<pi> :: perm
     assume "supp \<pi> \<sharp>* Terms.Let as body"
     ultimately
-    have *: "supp \<pi> \<sharp>* TransLet a  (PropLetHeap as body a) (map_transform (\<lambda>x0 x1. transform_sumC (x0, x1)) (PropLetHeap as body a) as) (transform_sumC (PropLetBody as body a, body))"
+    have *: "supp \<pi> \<sharp>* TransLet a  (PropLetHeap as body a) (map_transform (\<lambda>x0 x1. transform_sumC (x0, x1)) (PropLetHeap as body a) as) (transform_sumC (PropLetBody a, body))"
       by (auto simp add: fresh_star_def fresh_def)
 
-    have "TransLet a (PropLetHeap (\<pi> \<bullet> as) (\<pi> \<bullet> body) a) (map_transform (\<lambda>x0 x1. (\<pi> \<bullet> transform_sumC) (x0, x1)) (PropLetHeap (\<pi> \<bullet> as) (\<pi> \<bullet> body) a) (\<pi> \<bullet> as)) ((\<pi> \<bullet> transform_sumC) (PropLetBody (\<pi> \<bullet> as) (\<pi> \<bullet> body) a, \<pi> \<bullet> body)) = 
-        \<pi> \<bullet> (TransLet a (PropLetHeap as body a) (map_transform (\<lambda>x0 x1. transform_sumC (x0, x1)) (PropLetHeap as body a) as) (transform_sumC (PropLetBody as body a, body)))"
+    have "TransLet a (PropLetHeap (\<pi> \<bullet> as) (\<pi> \<bullet> body) a) (map_transform (\<lambda>x0 x1. (\<pi> \<bullet> transform_sumC) (x0, x1)) (PropLetHeap (\<pi> \<bullet> as) (\<pi> \<bullet> body) a) (\<pi> \<bullet> as)) ((\<pi> \<bullet> transform_sumC) (PropLetBody a, \<pi> \<bullet> body)) = 
+        \<pi> \<bullet> (TransLet a (PropLetHeap as body a) (map_transform (\<lambda>x0 x1. transform_sumC (x0, x1)) (PropLetHeap as body a) as) (transform_sumC (PropLetBody a, body)))"
        by (simp del: Let_eq_iff Pair_eqvt add:  eqvt_at_apply[OF goal18(2)])
-    also have "\<dots> = (TransLet a  (PropLetHeap as body a) (map_transform (\<lambda>x0 x1. transform_sumC (x0, x1)) (PropLetHeap as body a) as) (transform_sumC (PropLetBody as body a, body)))"
+    also have "\<dots> = (TransLet a  (PropLetHeap as body a) (map_transform (\<lambda>x0 x1. transform_sumC (x0, x1)) (PropLetHeap as body a) as) (transform_sumC (PropLetBody a, body)))"
       by (rule perm_supp_eq[OF *])
     also
     have "map_transform (\<lambda>x0 x1. transform_sumC (x0, x1)) (PropLetHeap (\<pi> \<bullet> as) (\<pi> \<bullet> body) a) (\<pi> \<bullet> as)
@@ -128,18 +131,40 @@ case (goal18 a as body a' as' body')
         apply (auto simp add: permute_self  dest: eqvt_at_apply''[OF goal18(1)[where aa = "(- \<pi> \<bullet> a)" for a], where p = \<pi>, symmetric])
         done
     moreover
-    have "(\<pi> \<bullet> transform_sumC) (PropLetBody (\<pi> \<bullet> as) (\<pi> \<bullet> body) a, \<pi> \<bullet> body) = transform_sumC (PropLetBody (\<pi> \<bullet> as) (\<pi> \<bullet> body) a, \<pi> \<bullet> body)"
+    have "(\<pi> \<bullet> transform_sumC) (PropLetBody a, \<pi> \<bullet> body) = transform_sumC (PropLetBody a, \<pi> \<bullet> body)"
       using eqvt_at_apply''[OF goal18(2), where p = \<pi>] by perm_simp
     ultimately
-    show "TransLet a (PropLetHeap (\<pi> \<bullet> as) (\<pi> \<bullet> body) a) (map_transform (\<lambda>x0 x1. transform_sumC (x0, x1)) (PropLetHeap (\<pi> \<bullet> as) (\<pi> \<bullet> body) a) (\<pi> \<bullet> as)) (transform_sumC (PropLetBody (\<pi> \<bullet> as) (\<pi> \<bullet> body) a, \<pi> \<bullet> body)) =
-          TransLet a (PropLetHeap as body a)   (map_transform (\<lambda>x0 x1. transform_sumC (x0, x1)) (PropLetHeap as body a) as) (transform_sumC (PropLetBody as body a, body))" by metis
+    show "TransLet a (PropLetHeap (\<pi> \<bullet> as) (\<pi> \<bullet> body) a) (map_transform (\<lambda>x0 x1. transform_sumC (x0, x1)) (PropLetHeap (\<pi> \<bullet> as) (\<pi> \<bullet> body) a) (\<pi> \<bullet> as)) (transform_sumC (PropLetBody a, \<pi> \<bullet> body)) =
+          TransLet a (PropLetHeap as body a)   (map_transform (\<lambda>x0 x1. transform_sumC (x0, x1)) (PropLetHeap as body a) as) (transform_sumC (PropLetBody a, body))" by metis
     qed
   qed auto
   nominal_termination by lexicographic_order
 end
 
+locale AbstractTransformSubst = AbstractTransform + AbstractAnalPropSubst +
+  assumes TransVar_subst: "(TransVar a v)[x ::= y] = (TransVar a v[x ::v= y])"
+  assumes TransVar1_subst: "(TransVar1 a v)[x ::= y] = (TransVar1 a v[x ::v= y])"
+  assumes TransApp_subst: "(TransApp a e v)[x ::= y] = (TransApp a e[x ::= y] v[x ::v= y])"
+  assumes TransLam_subst: "atom v \<sharp> (x,y) \<Longrightarrow> (TransLam a v e)[x ::= y] = (TransLam a v[x ::v= y] e[x ::= y])"
+  assumes TransLet_subst: "atom ` domA \<Gamma> \<sharp>* (x,y) \<Longrightarrow> (TransLet a ae \<Gamma> e)[x ::= y] = (TransLet a ae \<Gamma>[x ::h= y] e[x ::= y])"
+begin
+  lemma subst_transform: "(transform a e)[x ::= y] = transform a e[x ::= y]"
+  proof (nominal_induct e avoiding: x y arbitrary: a  rule: exp_strong_induct_set)
+  case (Let \<Delta> body x y)
+    hence *: "x \<notin> domA \<Delta>" "y \<notin> domA \<Delta>" by (auto simp add: fresh_star_def fresh_at_base)
+    hence "PropLetHeap \<Delta>[x::h=y] body[x::=y] a = PropLetHeap \<Delta> body a" by (rule PropLetHeap_subst)
+    with Let
+    show ?case
+    apply (auto simp add: fresh_star_Pair TransLet_subst simp del: Let_eq_iff)
+    apply (rule fun_cong[OF arg_cong[where f = "TransLet a b" for a b]])
+    apply (rule subst_map_transform)
+    apply simp
+    done
+  qed (case_tac b, simp_all add: TransVar_subst TransVar1_subst TransApp_subst TransLam_subst)
+end
+
 locale AbstractTransformBound = AbstractAnalProp + supp_bounded_transform  +
-  constrains PropApp :: "exp \<Rightarrow> var \<Rightarrow> 'a \<Rightarrow> 'a::pure_cont_pt"
+  constrains PropApp :: "'a \<Rightarrow> 'a::pure_cont_pt"
   constrains trans :: "'a::pure_cont_pt \<Rightarrow> exp \<Rightarrow> exp"
   assumes TransBound_eqvt: "\<pi> \<bullet> trans = trans"
 begin
@@ -159,8 +184,29 @@ begin
   apply (auto simp add: Let_supp supp_Pair supp_at_base dest: set_mp[OF supp_map_transform])[1]
   done
   qed
-
 end
 
+locale AbstractTransformBoundSubst = AbstractAnalPropSubst + AbstractTransformBound + 
+  assumes TransBound_subst: "(trans a e)[x::=y] = trans a e[x::=y]"
+begin
+  sublocale AbstractTransformSubst PropApp PropLam PropLetBody PropLetHeap
+      "(\<lambda> a. Var)"
+      "(\<lambda> a. Var1)"
+      "(\<lambda> a. App)"
+      "(\<lambda> a. Terms.Lam)"
+      "(\<lambda> a ae \<Gamma> e . Let (map_transform trans ae \<Gamma>) e)"
+  proof-
+  note PropApp_eqvt[eqvt_raw] PropLam_eqvt[eqvt_raw] PropLetBody_eqvt[eqvt_raw] PropLetHeap_eqvt[eqvt_raw] TransBound_eqvt[eqvt]
+  case goal1
+  show ?case
+  apply default
+  apply simp_all[4]
+  apply (simp del: Let_eq_iff)
+  apply (rule arg_cong[where f = "\<lambda> x. Let x y" for y])
+  apply (rule subst_map_transform)
+  apply (simp add: TransBound_subst)
+  done
+  qed
+end
 
 end
